separation.v
@@ -317,7 +317,7 @@ Proof. intros. by apply (sep_unmapped_difference x y). Qed.
 (** ** Properties of the [sep_unshared] predicate *)
 Lemma sep_unshared_valid x : sep_unshared x → sep_valid x.
 Proof. rewrite sep_unshared_spec'. by intros [??]. Qed.
-Lemma sep_unshared_unmapped x y : sep_unshared x → x ⊥ y → sep_unmapped y.
+Lemma sep_unshared_unmapped x y : x ⊥ y → sep_unshared x → sep_unmapped y.
 Proof. rewrite sep_unshared_spec'; naive_solver. Qed.
 Lemma sep_unshared_weaken x y : sep_unshared x → x ⊆ y → sep_unshared y.
 Proof.
@@ -826,10 +826,8 @@ Proof. induction 1; simpl; auto using sep_unmapped_valid. Qed.
 Lemma seps_unshared_valid xs : Forall sep_unshared xs → Forall sep_valid xs.
 Proof. induction 1; simpl; auto using sep_unshared_valid. Qed.
 Lemma seps_unshared_unmapped xs ys :
-  Forall sep_unshared xs → xs ⊥* ys → Forall sep_unmapped ys.
-Proof.
-  induction 2; decompose_Forall_hyps; eauto using sep_unshared_unmapped.
-Qed.
+  xs ⊥* ys → Forall sep_unshared xs → Forall sep_unmapped ys.
+Proof. induction 1; inversion_clear 1; eauto using sep_unshared_unmapped. Qed.
 Lemma seps_unshared_weaken xs ys :
   Forall sep_unshared xs → xs ⊆* ys → Forall sep_unshared ys.
 Proof.
